$ax^2 + bx + c = (x + d)^2 + e$

$0 = (x + d)^2 + e$

$-e = (x + d)^2$

$\sqrt{-e} = x + d$

$\sqrt{-e} - d = x$

----

$$(p + q)^2 = p^2 + 2pq + q^2$$

----

$$x^2 + \frac{bx}{a} + \frac{c}{a} = 0$$

$$x^2 + \frac{bx}{a} + (\frac{b}{2a})^2 + \frac{c}{a} = (\frac{b}{2a})^2$$

$$x^2 + \frac{bx}{a} + (\frac{b}{2a})^2 = (\frac{b}{2a})^2 - \frac{c}{a}$$

$$(x + \frac{b}{2a})^2 = (\frac{b}{2a})^2 - \frac{c}{a}$$

$$(x + \frac{b}{2a})^2 = \frac{b^2}{4a^2} - \frac{c}{a}$$

$$x + \frac{b}{2a} = \sqrt{\frac{b^2}{4a^2} - \frac{c}{a}}$$

$$x = -\frac{b}{2a} + \sqrt{\frac{b^2}{4a^2} - \frac{c}{a}}$$

$$x = -\frac{b}{2a} + \sqrt{\frac{b^2}{4a^2} - \frac{4c}{4a}}$$

$$x = -\frac{b}{2a} + \sqrt{\frac{b^2}{4a^2} - \frac{4ac}{4a^2}}$$

$$x = -\frac{b}{2a} + \sqrt{\frac{b^2 - 4ac}{4a^2}}$$

$$x = -\frac{b}{2a} + \frac{\sqrt{b^2 - 4ac}}{2a}$$

$$x = \frac{-b + \sqrt{b^2 - 4ac}}{2a}$$